{"nbformat":4,"nbformat_minor":0,"metadata":{"colab":{"name":"Q6.ipynb","provenance":[],"collapsed_sections":[],"authorship_tag":"ABX9TyMIkbhneSXI2E60MiicFHu7"},"kernelspec":{"name":"python3","display_name":"Python 3"},"language_info":{"name":"python"}},"cells":[{"cell_type":"code","metadata":{"id":"WskFs9pW1Yt4","colab":{"base_uri":"https://localhost:8080/"},"executionInfo":{"status":"ok","timestamp":1620479728736,"user_tz":-540,"elapsed":4785,"user":{"displayName":"Asha NDF","photoUrl":"https://lh3.googleusercontent.com/a-/AOh14Ghmk6UcXaYKgj2inQwOKS6s49TntUZgdmWo7mep=s64","userId":"14225296630148170886"}},"outputId":"aab4ebba-8964-4d4e-e34c-1e30f5bbc0c1"},"source":["S = input()\n","K = input()\n","C = 0\n","D = 1\n","S = S*int(K)\n","for i in range(1,len(S)):\n","  if S[i] =='?':\n","    D = D+1\n","  else:\n","    if S[i-1] =='?':\n","      D = D+1\n","    elif S[i] != S[i-1]:\n","      C = C+1\n","ans = 2**(D+1) + (2**D)*C -1\n","print(ans)"],"execution_count":4,"outputs":[{"output_type":"stream","text":["?1?\n","1\n","15\n"],"name":"stdout"}]}]}